Datalog/Reachable_Nodes.thy
@@ -58,7 +58,8 @@ next
     "q \<in> nodes_on_edge e"
     unfolding node_on_edge_list_def by auto
   then have "e = (q', l, q'') \<or> e \<in> set ((q'', l', q''') # ts)"
-    by (metis (no_types, lifting) append_Cons hd_append in_set_conv_decomp list.sel(1) list.sel(3) tl_append2)
+    by (metis (no_types, lifting) append_Cons hd_append in_set_conv_decomp list.sel(1) list.sel(3) 
+        tl_append2)
   then show ?case
   proof 
     assume "e = (q', l, q'')"
@@ -79,7 +80,8 @@ next
   next
     assume "e \<in> set ((q'', l', q''') # ts)"
     then have "q \<in> bw_may.S_hat_edge_list ((q'', l', q''') # ts) d_init_RN"
-      by (metis "2.IH" "2.hyps"(2) "2.prems"(2) \<open>q \<in> nodes_on_edge e\<close> append_Cons append_Nil in_set_conv_decomp last.simps list.distinct(1) node_on_edge_list_def)
+      by (metis "2.IH" "2.hyps"(2) "2.prems"(2) \<open>q \<in> nodes_on_edge e\<close> append_Cons append_Nil 
+          in_set_conv_decomp last.simps list.distinct(1) node_on_edge_list_def)
     then show ?case
       unfolding bw_may.S_hat_edge_list.simps bw_may.S_hat_def by auto
   qed
@@ -117,13 +119,16 @@ next
       assume "\<pi> = []"
       then show "node_on_edge_list (e # \<pi>) q"
         using d_init_RN_def q_Shat
-        by (metis Cons.prems(2) Diff_empty append.left_neutral append_Cons bw_may.S_hat_edge_list.simps(1) insertI1 insert_commute kill_set_RN.elims last_ConsL nodes_on_edge.elims node_on_edge_list_def singleton_iff trans_tl.simps)   
+        by (metis Cons.prems(2) Diff_empty append.left_neutral append_Cons 
+            bw_may.S_hat_edge_list.simps(1) insertI1 insert_commute kill_set_RN.elims last_ConsL 
+            nodes_on_edge.elims node_on_edge_list_def singleton_iff trans_tl.simps)   
  qed
   next
     assume "q \<in> gen_set_RN e"
     then show ?thesis
       unfolding node_on_edge_list_def
-      by (metis append.left_neutral append_Cons empty_iff gen_set_RN.elims insert_iff nodes_on_edge.simps)
+      by (metis append.left_neutral append_Cons empty_iff gen_set_RN.elims insert_iff 
+          nodes_on_edge.simps)
   qed
 qed
 
