Datalog/Very_Busy_Expressions.thy
@@ -7,7 +7,9 @@ theory Very_Busy_Expressions imports Available_Expressions begin
 section \<open>Very Busy Expressions\<close>
 
 definition vbexp_edge_list :: "('n,'v action) edge list \<Rightarrow> 'v arith \<Rightarrow> bool" where
-  "vbexp_edge_list \<pi> a = (\<exists>\<pi>1 \<pi>2 e. \<pi> = \<pi>1 @ [e] @ \<pi>2 \<and> a \<in> aexp_edge e \<and> (\<forall>e' \<in> set \<pi>1. fv_arith a \<inter> def_edge e' = {}))"
+  "vbexp_edge_list \<pi> a = (\<exists>\<pi>1 \<pi>2 e. \<pi> = \<pi>1 @ [e] @ \<pi>2 \<and> 
+                                    a \<in> aexp_edge e \<and> 
+                                    (\<forall>e' \<in> set \<pi>1. fv_arith a \<inter> def_edge e' = {}))"
 
 definition vbexp_path :: "'n list \<times> 'v action list \<Rightarrow> 'v arith set" where
   "vbexp_path \<pi> = {a. vbexp_edge_list (LTS.transition_list \<pi>) a}"
